\documentclass{article}

\usepackage{fancyhdr}
\usepackage{extramarks}
\usepackage{amsmath}
\usepackage{amsthm}
\usepackage{amsfonts}
\usepackage{tikz}
\usepackage[plain]{algorithm}
\usepackage{algpseudocode}
\usepackage{chngcntr}
\usepackage{mathtools}
\usepackage[utf8]{inputenc}
\usepackage[english]{babel}
\usepackage{thmtools}
\usepackage{mathrsfs}
\usepackage{enumitem}

\declaretheoremstyle[headfont=\scshape,postheadspace=\newline]{mystyle}
\declaretheorem[style=mystyle]{theorem}

\usetikzlibrary{automata,positioning}

%
% Basic Document Settings
%

\topmargin=-0.45in
\evensidemargin=0in
\oddsidemargin=0in
\textwidth=6.5in
\textheight=9.0in
\headsep=0.25in

\linespread{1.1}

\pagestyle{fancy}
\lhead{\hmwkAuthorName}
\chead{\hmwkTitle}
\rhead{\firstxmark}
\lfoot{\lastxmark}
\cfoot{\thepage}

\renewcommand\headrulewidth{0.4pt}
\renewcommand\footrulewidth{0.4pt}

\setlength\parindent{0pt}

%\newtheorem{theorem}{Theorem}[section]
\newtheorem{corollary}{Corollary}[theorem]
\newtheorem{lemma}[theorem]{Lemma}
\theoremstyle{definition}
\newtheorem{definition}{Definition}[section]


%
% Create Problem Sections
%

\newcommand{\enterProblemHeader}[1]{
}

\newcommand{\exitProblemHeader}[1]{
    \nobreak\extramarks{#1 (continued)}{#1 continued on next page\ldots}\nobreak{}
    \stepcounter{#1}
    \nobreak\extramarks{#1}{}\nobreak{}
}

\setcounter{secnumdepth}{0}
\newcounter{partCounter}
\newcounter{homeworkProblemCounter}
\setcounter{homeworkProblemCounter}{1}

%
% Homework Problem Environment
%
% This environment takes an optional argument. When given, it will adjust the
% problem counter. This is useful for when the problems given for your
% assignment aren't sequential. See the last 3 problems of this template for an
% example.
%
\newenvironment{homeworkProblem}[1]{
    \section{#1}
    \setcounter{partCounter}{1}
    \setcounter{equation}{0}
    \setcounter{theorem}{0}
}

%
% Homework Details
%   - Title
%   - Due date
%   - Class
%   - Section/Time
%   - Instructor
%   - Author
%

\newcommand{\hmwkTitle}{MATH 2A: Differential Equations}
\newcommand{\hmwkDueDate}{}
\newcommand{\hmwkClass}{Discrete Mathematics}
\newcommand{\hmwkClassTime}{}
\newcommand{\hmwkClassInstructor}{}
\newcommand{\hmwkAuthorName}{\textbf{Edwin Njinimbam}}

%
% Title Page
%

\title{
    \vspace{2in}
    \textmd{\textbf{\hmwkClass\ \hmwkTitle}}\\
    \vspace{0.1in}\large{\textit{\hmwkClassInstructor\ \hmwkClassTime}}
    \vspace{3in}
}

\author{\hmwkAuthorName}
\date{}

\renewcommand{\part}[1]{\textbf{\large Part \Alph{partCounter}}\stepcounter{partCounter}\\}

%
% Various Helper Commands
%

% Useful for algorithms
\newcommand{\alg}[1]{\textsc{\bfseries \footnotesize #1}}

% For derivatives
\newcommand{\deriv}[2]{\frac{\mathrm{d}{#1}}{\mathrm{d}{#2}}}
\newcommand{\derivs}[2]{\frac{\mathrm{d}^2 {#1}}{\mathrm{d}{#2}^2}}

% For partial derivatives
\newcommand{\pderiv}[2]{\frac{\partial #1}{\partial #2}}
\newcommand{\pderivs}[2]{\frac{\partial^2 #1}{\partial #2^2}}

% Integral dx
\newcommand{\dx}{\mathrm{d}x}

% Alias for the Solution section header
\newcommand{\solution}{\textbf{\large Solution}}

% Probability commands: Expectation, Variance, Covariance, Bias
\newcommand{\E}{\mathrm{E}}
\newcommand{\Var}{\mathrm{Var}}
\newcommand{\Cov}{\mathrm{Cov}}
\newcommand{\Bias}{\mathrm{Bias}}

\newcommand{\ls} {\(\mathcal{LS}(A,\textbf{0})\)}
\newcommand{\nullspace}[1]{\mathcal{N}(#1)}
\newcommand{\p} {$\boxed{1}$~}
\newcommand*\Domain[1]{\in\mathbb{C}^{#1}}
\newcommand{\iu}{{i\mkern1mu}}

\counterwithin*{equation}{section}
\counterwithin*{equation}{subsection}

\newcommand{\matxx}[2] {
\begin{bmatrix}
  #1 \\
  #2 \\
\end{bmatrix}
}

\newcommand{\matxxx}[3] {
\begin{bmatrix}
  #1 \\
  #2 \\
  #3 \\
\end{bmatrix}
}

\newcommand{\matxxxx}[4] {
\begin{bmatrix}
  #1 \\
  #2 \\
  #3 \\
  #4 \\
\end{bmatrix}
}
\newcommand{\matxxxxx}[5] {
\begin{bmatrix}
  #1 \\
  #2 \\
  #3 \\
  #4 \\
  #5 \\
\end{bmatrix}
}

\newcommand{\matxxxxxx}[6] {
\begin{bmatrix}
  #1 \\
  #2 \\
  #3 \\
  #4 \\
  #5 \\
  #6 \\
\end{bmatrix}
}

\newcommand{\arrow}[1] {\xrightarrow[]{\text{#1}}}

\newcommand{\specialcell}[2][c]{%
  \begin{tabular}[#1]{@{}c@{}}#2\end{tabular}}

\newenvironment{solutionToProblem} {

  \bigskip

  \textbf{Solution}
}

\begin{document}

\pagebreak

\begin{homeworkProblem}{Chapter 1 B: Picard's Method}
  \begin{enumerate}[label=(\alph*)]
  \item  Use Picard's method with \(\psi_{0}(x) = 1\) to obtain the next four
    successive approximations of the solution to
    \[y^{\prime}(x) = y(x), \hspace{0.5cm} y(0) = 1\]
    Show that these approximations are just the partial sums of the Maclaurin
    series for the actual solution \(e^x\).

    \begin{solutionToProblem}
      Given that
      \begin{equation}
        y^{\prime}(x) = y(x), \hspace{0.5cm} y(0) = 1
      \end{equation}

      Also given that
      \begin{equation}
        f(x,y) = y(x)
      \end{equation}
      According to picards theorem, we have
      \begin{equation}
        \begin{split}
          \phi_{n+1}(x) & = y_0 + \int^{x}_{x_{0}}{f(t, \phi_{0}(t))}dt \\
          & = 1 + \int^{x}_{0}{1}dt \\
          & = 1 + x
        \end{split}
      \end{equation}

      \begin{equation}
        \begin{split}
          \phi_{2}(x) & = y_0 + \int^{x}_{0}f(t, \phi_1(t))dt \\
          & = 1 + \int^{x}_{0} f(t, \left( 1+t \right))dt \\
          & = 1 + x + \frac{x^2}{2}
        \end{split}
      \end{equation}

      \begin{equation}
        \begin{split}
          \phi_{3}(x) & = y_0 + \int^{x}_{0}f(t, \phi_2(t))dt \\
          & = 1 + \int^{x}_{0} f \left(t, \left( 1+t + \frac{t^2}{2} \right) \right)dt \\
          & = 1 + x + \frac{x^2}{2} + \frac{x^3}{6}
        \end{split}
      \end{equation}

      \begin{equation}
        \begin{split}
          \phi_{4}(x) & = y_0 + \int^{x}_{0}f(t, \phi_3(t))dt \\
          & = 1 + \int^{x}_{0}f \left( t, \left( 1 + t + \frac{t^2}{2} \right) \right)dt \\
          & = 1 + x + \frac{x^2}{2} + \frac{x^3}{6} + \frac{x^4}{24}
        \end{split}
      \end{equation}

      By observing the pattern as \(n\) goes, it is enough to say that
      \[
        \phi_{n}(x) = 1 + x + x^2 + \frac{x^2}{2} + \frac{x^3}{6} + \dots + \frac{x^n}{n!}
      \]

      This is the partial sum of the Maclaurian series of \(e^x\).
    \end{solutionToProblem}

  \item Use Picard's method with \(\psi+{0}(x) = 0\) to obtain the next
    three successive approximations of the solution to the nonlinear problem
    \[
      y^{\prime}(x) = 3x - \left[ y(x)^2 \right], \hspace{0.5cm} y(0) = 0
    \]
    Graph these approximations for \(0 \leq x \leq 1\).

    \begin{solutionToProblem}
      \setcounter{equation}{0}
      \begin{equation}
        \begin{split}
          y(x_1) & = y(x_0) + \int^{x}_{x_0}{f(x,y)dx} \\
          & = f(x,y) = 2x - y^2 \\
          y(0) & = 0
        \end{split}
      \end{equation}
      We assume that \(x_0 = 0, x_1 = 0.25\) then
      \begin{equation}
        \begin{split}
          \phi_1(x) & = y(0) + \int^{x}_{0}{\phi_0(x)dx} = 0 + \int^{x}_{0}{2x - 0}dx = x^2 \\
          \phi_2(x) & = y(0) + \int^{x}_{0}{\phi_1(x)dx} = 0 + \int^{x}_{0}{(2x - x^2)dx} = x^2 - =frac{x^3}{3} \\
          \phi_3(x) & = y(0) + \int^{x}_{0}{\phi_2(x)dx} = 0 + \int^{x}_{0}{(2x - x^2 + \frac{x^3}{3})dx} = x^2 - =frac{x^3}{3} + \frac{x^4}{12} \\
          \phi_4(x) & = y(0) + \int^{x}_{0}{\phi_3(x)dx} = 0 + \int^{x}_{0}{(2x - x^2 + \frac{x^3}{3} - \frac{x^4}{12})dx} = x^2 - =frac{x^3}{3} + \frac{x^4}{12} - \frac{x^5}{60} \\
        \end{split}
      \end{equation}
      If \(x = 0.25, \phi_1(x) = 0.0625, \phi_2(x) = 0.05729, \phi_3(x) =
      0.05761, \phi_4(x) = 0.0576009\).
      Thus, the better approximationn at \(x = 0.25\) is \(0.0576\).

      If \(x = 0.5, \phi_1(x) = 0.25, \phi_2(x) = 0.2083, \phi_3(x) =
      0.203125, \phi_4(x) = 0.21302\).

      If \(x = 0.75, \phi_1(x) = 0.5625, \phi_2(x) = 0.421875, \phi_3(x) =
      0.44824, \phi_4(x) = 0.605419\).

      \begin{center}
        \begin{figure}[h!]
          \includegraphics[width=7cm]{chap1b.jpg}
          \caption{}
          \label{fig:chap1b}
        \end{figure}
      \end{center}
    \end{solutionToProblem}

  \item In Problem 29 in Exercises 1.2, we showed that the initial value
    problem
    \[y^{\prime}(x) = 3\left[ y(x)\right]^{2/3}, y(2) = 0\]
    does not have a unique solution. Show that Picard's method beginning
    with \(\psi_{0}(x) = 0\) converges to the solution \(y(x) = 0\),
    whereas Picard's method beginning with \(\psi_{0}(x) = x - 2\)
    converges to the second solution \(y(x) = (x - 2)^{3}\).

    \begin{solutionToProblem}
      \setcounter{equation}{0}
      The given IVP can be written as
      \begin{equation}
        y^{\prime}(t) = f(x, y(x)) \mbox{ where } f(x,y(x)) = 3(y(x))^{2/3}
      \end{equation}

      The first iteration is given by

      \begin{equation}
        \begin{split}
          y_1(x) & = y(2) + \int^{x}_{2} f(u, y(2))du \\
          & = 0 + \int^{t}_{2} f(u, 0)du \\
          & = 0 + \int^{x}_{0} 0du = 0
        \end{split}
      \end{equation}
      If we repeat the procedure, then we get
      \begin{equation}
        y_2(x) = 0
      \end{equation}

      Thus, we get the trivial solution \(y(x) = 0\) for the IVP.

      \bigskip

      Suppose that
      \begin{equation}
        \phi_0(x) = x - 2
      \end{equation}

      Then the first iteration is given by
      \begin{equation}
        \begin{split}
          \phi_1(x) & = \phi_0(x) + \int^{x}_{2} f\left( u, \phi_0(x) \right)du \\
          & = x - 2 + \int^{x}_{2}f(u, x-2)du \\
          & = x - 2 + \int^{x}_{2}{3(x - 2)^{2/3}du} = x - 2 3 \frac{(x-2)^{5/3}}{5/3} \Bigm|_2^x \\
          & = x - 2 + \frac{9}{5}(x-2)^{5/3} = (x-2)\left( 1 + \frac{9}{5}(x-2)^{2/3} \right)
        \end{split}
      \end{equation}

      The second iteration is given by
      \begin{equation}
        \begin{split}
          \phi_2(x) & = \phi_0(x) + \int^{x}_{2}{\left( fu, \phi_1(x) \right)du} \\
          & = x - 2 + \int^{x}_{2}f\left( u, x-2 \right)du \\
          & = x - 2 + \int^{x}_{2}{x - 2 + \frac{9}{5}(x-2)^{5/3}du} = x - 2 + \left( \frac{(x-2)^2}{2} + \frac{9}{5}\frac{(x-2)^{8/3}}{8/3} \Bigm|^{x}_{2} \right) \\
          & = x - 2 =\frac{(x-2)^{2}}{2} + \frac{27}{40}(x-2)^{8/3}
        \end{split}
      \end{equation}
    \end{solutionToProblem}
  \end{enumerate}
\end{homeworkProblem}

\pagebreak

\begin{homeworkProblem}{The Phase Line}
  \begin{enumerate}[label=(\alph*)]
  \item The slopes in the direction field are all identical along horizontal
    lines.

    \begin{solutionToProblem}
    \end{solutionToProblem}
    
  \item New solutions can be generated from old ones by time shifting [i.e.,
    replacing \(y(t)\) with \(y(t-t_0)\).]

    \begin{solutionToProblem}
    \end{solutionToProblem}
        
  \item Sketch the phase line for \(y^{\prime} = (y - 1)(y - 2)(y - 3)\) and
    state the nature of its equilibria.

    \begin{solutionToProblem}
    \end{solutionToProblem}
    
  \item Use the phase line for \(y^{\prime} = -(y - 1)^{5/3}(y - 2)^2(y -
    3)\) to predict the asymtotic behavior as \(t \rightarrow \infty\) of the
    solution satisfying \(y(0) = 2.1\).
    \begin{solutionToProblem}
    \end{solutionToProblem}
    
  \item Sketch the phase line for \(y^{\prime} = y{\sin{y}}\) and state the
    nature of its equilibria.
    \begin{solutionToProblem}
    \end{solutionToProblem}
    
  \item Sketch the phase lines for \(y^{\prime} = y \sin{y} + 0.1\) and
    \(y^{\prime} = y\sin{y} - 0.1\). Discuss the effect of the small
    perturbation \(\pm 0.1\) on the equilibria.
    \begin{solutionToProblem}
    \end{solutionToProblem}
  \end{enumerate}
\end{homeworkProblem}

\pagebreak

\begin{homeworkProblem}{Chapter 4 A: Nonlinear Equations Solvable by First-Order Techniques}
  \begin{enumerate}[label=(\alph*)]
  \item
    \begin{solutionToProblem}
      
      The given equation can ben rewritten as
      
      \[
        \begin{split}
          2x\deriv{w}{x} - w + \frac{1}{w} & = 0 \\
          2x\deriv{w}{x} & = w - \frac{1}{w} \\
          \frac{1}{w - 1/w}dw & = \frac{1}{2x}dx
        \end{split}
      \]

      Therefore we get
      \[
        \frac{1}{2} \int{\left( \frac{1}{w^2 - 1}2w \right) dw} = \frac{1}{2} \int{\frac{1}b{2}dx}
      \]

      That is
      \[
        \begin{split}
          \ln{w^2 - 1} & = \ln{\left| x \right| + C} \\
          w^2 - 1 & = x + C \\
          w & = \deriv{y}{x} = \sqrt{x + 1}
        \end{split}
      \]

      Thus, we obtain

      \[
        y = \int{\left( x + 1 \right)^{\frac{1}{2}}}dx = \frac{1}{2\sqrt{x+1}} + C
      \]
    \end{solutionToProblem}
  \item
    
    \begin{solutionToProblem}
      \[
        \begin{split}
          (2y)(w)\deriv{w}{y} & = 1 + w^2 \\
          2y\deriv{w}{y} & = \frac{1}{w} + w = \frac{w^2 + 1}{w} \\
        \end{split}
      \]

      This becomes
      \[
        \frac{1}{2}\int{1}{\left( w^2 + 1 \right) (2w)dw} = \frac{1}{2} \int{\frac{1}{y}}dy
      \]

      Then we obtain
      \[
        \begin{split}
          w & = \sqrt{y - 1} + C
        \end{split}
      \]

      \[
        \begin{split}
          \int{\frac{1}{\sqrt{y - 1}}dy} = \int{dx}
          \sqrt{y - 1} & = 2x + C_1
        \end{split}
      \]

      Thus we obtain
      \[
        y_1 = 1 + 4x^2 + C
      \]

      Then we need to have another equation.
      \[
        2yw\deriv{w}{y} = -yw
        2\deriv{w}{y} = -\frac{yw}{yw} = -1
      \]

      \[
        \begin{split}
          \int{dw} & = -\frac{1}{2}\int{dy} \\
          -2 \int{\frac{1}{y}dy} & = \int{dx}
        \end{split}
      \]

      This becomes
      \[
        \begin{split}
          -2\ln{\left| y \right|} & = x + C \\
          \ln{\left| y \right|} & = -\frac{1}{2}x + C
        \end{split}
      \]

      Thus, we get
      \[
        y_2 = Ce^{-\frac{x}{2}}
      \]
    \end{solutionToProblem}

  \item \textbf{Suspended Cable.}
    \begin{solutionToProblem}
      \setcounter{equation}{0}
      The given differential equation is
      \begin{equation}
        y^{\prime\prime} = \frac{1}{a}\sqrt{1 + \left( \deriv{y}{x} \right)^2}; \hspace{0.5cm} y(0) = a, \hspace{0.5cm} y^{\prime}(0) = 0, \hspace{0.2cm} \mbox{ where } a (\neq 0) \mbox{ is a constant.}
      \end{equation}

      Let \(v = y^{\prime}\) then we can say that \(\deriv{v}{x} =
      y^{\prime\prime}\)
      
      Now, we solve
      \begin{equation}
        \begin{split}
          \deriv{v}{x} & = \frac{1}{a}\sqrt{1 + v^2} \\
          \int{\frac{dv}{\sqrt{1 + v^2}}} & = a\int{dx} \\
        \end{split}
      \end{equation}

      This becomes
      \begin{equation}
        \ln{\sqrt{1+v^2} + v} = ax
      \end{equation}

      Thus, this is enough reason to say that
      \[
        \begin{split}
          x^{\prime}(0) & = 0 \\
        \end{split}
      \]
      This means \(C = 0\).

      Therefore

      \begin{equation}
        \begin{split}
          \ln{\sqrt{1 + v^2} + v} & = ax \\
          \sqrt{1 + v^2} + v & = e^{ax} \\
          \left( -\sqrt{1 + v^2} \right) & = \left( v - e^{ax} \right)^2 \\
          v & = \frac{e^{2ax} - 1}{2e^{ax}} = \frac{1}{2}\left[ e^{ax} - e^{-ax}\right]
        \end{split}
      \end{equation}

      \begin{equation}
        \begin{split}
          \deriv{y}{x} & = \frac{1}{2}\left( e^{ax} - e^{-ax}\right) \\
          \int{dy} & = \frac{1}{2}\int{\left( e^{ax} - e^{-ax} \right)dx} \\
          y & = \frac{1}{2}\frac{\left( e^{ax} + e^{-ax} \right)}{a} + C_2
        \end{split}
      \end{equation}

      At \(y(0) = a\),
      \[
        a = \frac{1}{2}\frac{2}{a} + C_2
      \]

      Therefore,
      \[
        C_2 = \frac{\left( a^2 - 1 \right)}{a}
      \]

      Then finally we get
      \begin{equation}
        y = \frac{1}{2}\left( \frac{a^{ax} + e^{-ax}}{a} \right) + \frac{a^2 - 1}{a}
      \end{equation}
    \end{solutionToProblem}
  \end{enumerate}
\end{homeworkProblem}

\pagebreak

\begin{homeworkProblem}{Chapter 4C: Simple Pendulum}
  \begin{enumerate}[label=(\alph*)]
  \item
    \begin{solutionToProblem}
      By assuming the problem consisting of mass \(m\) suspended by a rod of
      length \(l\) and writing the derived nonlinear initial value problem,
      \[
        \derivs{\theta}{t} + \frac{g}{l} \sin{\theta} = 0, \hspace{0.5cm}
        \theta(0) = \alpha(0), \theta^{\prime}(0) = 0
      \]

      Let us determine the equation of motion for the pendulum and its period.

      \begin{equation}
        \begin{split}
          \left( \deriv{\theta}{t} \right) \left( \derivs{\theta}{t} \right) + \frac{g}{l} \sin{\theta}\left( \deriv{\theta}{t} \right) & = 0 \\
          \deriv{}{t} \left( \frac{1}{2} \left( \deriv{\theta}{t} \right)^2 - \frac{g}{l} \cos{\theta} \right) & = 0 \\
          \frac{1}{2} \left( \deriv{\theta}{t} \right)^2 - \frac{g}{l} \cos{theta} & = c \\
          \left( \frac{\theta}{t} \right)^2 - \frac{2g}{l} \cos{\theta} = C
        \end{split}
      \end{equation}

      By applying the initial conditions,
      \begin{equation}
        \left( \theta^{\prime}(0) \right)^2 - \frac{2g}{l}\cos{theta}(0) = C
      \end{equation}

      Then we get
      \begin{equation}
        \begin{split}
          0 - \frac{2g}{l} \cos{\alpha} & = C \\
          C & = - \frac{2g}{l} \cos{\alpha}
        \end{split}
      \end{equation}

      By substituting \(C\) value into \(\left( \deriv{\theta}{t} \right)^2 -
      \frac{2g}{l} \cos{\theta} = C\), then we get
      \begin{equation}
        \begin{split}
          \left( \deriv{\theta}{t} \right)^2 - \frac{2g}{l} \cos{\theta} & = - \frac{2g}{l} \cos{\alpha} \\
          \left( \deriv{\theta}{t} \right)^2 & = \frac{2g}{l}\left( \cos{\theta} - \cos{\alpha} \right) \\
          \deriv{\theta}{t} & = - \sqrt{\frac{2g}{l} \left( \cos{\theta} - \cos{\alpha} \right)} \\
          dt & = - \sqrt{\frac{1}{2g}} \frac{d\theta}{\sqrt{\left( \cos{\theta} - \cos{\alpha} \right)}}
          \end{split}
      \end{equation}
    \end{solutionToProblem}

  \item
    \begin{solutionToProblem}
      By using the formula, \(\cos{x} = 1 - 2\sin^2{x}\), we can say that
      \begin{equation}
        \begin{split}
          dt & = - \sqrt{\frac{1}{2g}} \frac{d\theta}{\sqrt{\left( \left( 1 - 2\sin^2{\theta} \right) - \left( 1 - 2\sin^2{\alpha} \right) \right)}} \\
          dt & = - \frac{1}{2}\sqrt{\frac{l}{g}} \frac{d\theta}{\sqrt{sin^2{\frac{\alpha}{2}} - \sin^2{\frac{\theta}{2}}}}
        \end{split}
      \end{equation}
    \end{solutionToProblem}

  \item
    \begin{solutionToProblem}
      Now, let us determine the elapsed time \(T\), for the pendulum to fall
      from the angle \(\theta = \alpha\) to the angle \(\theta = \beta\)
      corresponding to \(\phi = \frac{\pi}{2}\) to \(\phi = \Phi\)

      \begin{equation}
        \begin{split}
          T = \int^{t}_0{dt} & = - \frac{1}{2} \sqrt{\frac{l}{g}} \frac{d\theta}{\sqrt{\sin^2{\frac{\alpha}{2}} - \sin^2{\frac{\theta}{2}}}} \\
          & = - \frac{1}{2} \sqrt{\frac{l}{g}} \int^{\phi}_{\frac{\pi}{2}}{\frac{d\theta}{\sqrt{\sin^2{\frac{\alpha}{2}} - \sin^2{\frac{\theta}{2}}}}} \\
          & = - \sqrt{\frac{l}{g}} \int^{\phi}_{\frac{\pi}{2}}{\frac{d\phi}{\sqrt{1 - k^2 \sin^2{\phi}}}}, \hspace{0.3cm} \mbox{ where } k = \sin{\frac{\alpha}{2}}
        \end{split}
      \end{equation}

      Thus, we get
      \begin{equation}
        -T = \sqrt{\frac{1}{g}} \int^{\phi}_{\frac{\pi}{2}}{\frac{d\phi}{1 - k^2 \sin^2{\phi}}}
      \end{equation}
    \end{solutionToProblem}
  \item
    \begin{solutionToProblem}
      Let us determine the period \(P\) of the pendulum.
      The period is defined to be the time required for it swing from one
      extreme to other extreme and back. Therefore, from \(\alpha\) to
      \(-\alpha\) and from \(-\alpha\) to \(\alpha\).
      Therefore, the total period is four equal parts.
      Thus, the period is given by

      \begin{equation}
        P = (4) \sqrt{\frac{l}{g}} \int^{\frac{\pi}{2}}_{0}{\frac{d\phi}{\sqrt{1 - k^2 \sin^2{\phi}}}}
      \end{equation}

      Now, the integral
      \[
        \int^{\frac{\pi}{2}}_{0}{\frac{d\phi}{\sqrt{1 - k^2 \sin^2(\phi)}}}
      \]
      is called an elliptic integral of the first kind and denoted by
      \[
        F\left( k, \frac{\pi}{2} \right) =
        \int^{\frac{\pi}{2}}_{0}{\frac{d\phi}{\sqrt{1 - k^2 \sin^2{\phi}}}}
      \]
    \end{solutionToProblem}
  \item
    \begin{solutionToProblem}
      \begin{equation}
        \begin{split}
          \frac{P}{4} + (-T) & = \sqrt{\frac{l}{g}} \int^{\frac{\pi}{2}}_{0}{\frac{d\phi}{\sqrt{1 - k^2 \sin^2(\phi)}}} + \sqrt{\frac{l}{g}} \int^{\phi}_{\frac{\pi}{2}}{\frac{d\phi}{\sqrt{1 - k^2 \sin^2(\phi)}}} \\
          -T + \frac{P}{4} & = \sqrt{\frac{l}{g}} \int^{\phi}_{0}{\frac{d\phi}{\sqrt{1 - k^2 \sin^2{\phi}}}} \\
          -T + \frac{P}{4} & = \sqrt{\frac{l}{g}}F \left( k, \Phi \right)
        \end{split}
      \end{equation}

      This is obtained by substituting
      \[
        F \left( k, \Phi \right) = \int^{\phi}_{0}{\frac{d\phi}{\sqrt{1 - k^2 \sin^2{\phi}}}}
      \]
    \end{solutionToProblem}
  \end{enumerate}
\end{homeworkProblem}

\pagebreak

\begin{homeworkProblem}{Linearization of Nonlinear Problems}
  \begin{enumerate}[label=(\alph*)]
  \item
    \begin{solutionToProblem}
      \begin{equation}
        \begin{split}
          \theta^{\prime}(t) & = -\sin{\theta(t)} \\
          \theta^{\prime\prime}(0) & = -\sin(\theta(0)) \\
          \theta^{\prime\prime\prime}(t) & = -\cos{\theta(t)}\theta^{\prime}(t) \\
          \theta^{(4)} & = \sin(\theta(t))(\theta^{\prime}(t))^2 - \cos(\theta(t))\theta^{\prime\prime}(t) \\
        \end{split}
      \end{equation}

      \[
        \theta^{(4)}(0) = \sin{\theta(0)}(\theta^{\prime}(0))^2 + \cos(\theta(0))\sin(\theta(0))
      \]

      \[
        \theta^{(5)}(t) = \cos(\theta(t))(\theta^{\prime}(t))^3 +
        2\sin(\theta(t))\theta^{\prime}(t)\theta^{\prime\prime}(t) +
        \deriv{ \left(  \sin{2\theta(t)} \right) }{t} \left( \frac{1}{2} \right)
      \]

      \[
        \begin{split}
                  \theta^{(5)}(t) & = \cos(\theta(t))(\theta^{\prime}(t))^3 +
                  2\sin{\theta(t)} \theta^{\prime}(t) \theta{^\prime\prime}(t) +
                  \cos{2\theta(t)}\theta^{\prime}(t) \\
                  \theta^{(5)}(0) & = \cos(\theta(0))(\theta^{\prime}(0))^3 +
                  2\sin{\theta(0)} \theta^{\prime}(0) \theta{^\prime\prime}(0) +
                  \cos{2\theta(0)}\theta^{\prime}(0) \\
        \end{split}
      \]
    \end{solutionToProblem}
  \item
    \begin{solutionToProblem}
      \[
        derivs{\theta}{t} + \theta = 0
      \]

      Now solving for \(\theta\), then we get
      \[
        \begin{split}
          \theta & = C_1e^t + C_2e^{-t} \\
          \theta(0) & = C_1 + C_2 = \frac{\pi}{2}
        \end{split}
      \]

      Since
      \[
        \theta^{\prime}(t) = C_1e^{t} - C_2e^{-t}
      \]

      The constant values are
      \[
        \begin{split}
          C_1 - C_2 & = 0 \\
          C_1 = C_2 = \frac{\pi}{24}
        \end{split}
      \]

      Thus,
      \[
        \theta(t) = \frac{\pi}{24}\left[ e^t + e^{-t} \right]
      \]
    \end{solutionToProblem}

  \item
    \begin{solutionToProblem}
    \end{solutionToProblem}

  \item
    \begin{solutionToProblem}
    \end{solutionToProblem}

  \item
    \begin{solutionToProblem}
    \end{solutionToProblem}
  \end{enumerate}
\end{homeworkProblem}
\end{document}
